Integrated loads of additional state laws

robochart/untimed/Actions.thy
@@ -4,49 +4,6 @@ theory Actions
   imports ReactiveSpec
 begin
 
-lemma st_post_CRR [closure]: "[b]\<^sub>S\<^sub>> is CRR"
-  by (rel_auto)
-
-lemma st_post_unrest_ref' [unrest]: "$ref\<acute> \<sharp> [b]\<^sub>S\<^sub>>"
-  by (rel_auto)
-
-definition StateInvC :: "'s upred \<Rightarrow> ('s, 'e) action" ("sinv\<^sub>C'(_')") where
-[rdes_def]: "sinv\<^sub>C(b) = \<^bold>R\<^sub>s([b]\<^sub>S\<^sub>< \<turnstile> true\<^sub>r \<diamondop> [b]\<^sub>S\<^sub>>)"
-
-lemma StateInvC_NCSP [closure]: "sinv\<^sub>C(b) is NCSP"
-  by (simp add: StateInvC_def closure unrest)
-
-lemma CACT_rdes_intro:
-  assumes "P\<^sub>1 is CRC" "P\<^sub>2 is CRR" "P\<^sub>2 is CDC" "P\<^sub>3 is CRR" "$st\<acute> \<sharp> P\<^sub>2" "$ref\<acute> \<sharp> P\<^sub>3"
-  shows "\<^bold>R\<^sub>s (P\<^sub>1 \<turnstile> P\<^sub>2 \<diamondop> P\<^sub>3) is CACT"
-  by (rule CACT_intro, simp add: closure assms, rule C2_rdes_intro, simp_all add: assms)
-
-lemma StateInvC_CACT [closure]: "sinv\<^sub>C(b) is CACT"
-  by (simp add: CACT_rdes_intro rdes_def closure unrest)
-
-lemma StateInvC_seq_idem:
-  "sinv\<^sub>C(b) ;; sinv\<^sub>C(b) = sinv\<^sub>C(b)"
-  by (rdes_eq)
-
-lemma StateInvC_seq_refine:
-  assumes "sinv\<^sub>C(b) \<sqsubseteq> P" "sinv\<^sub>C(b) \<sqsubseteq> Q"
-  shows "sinv\<^sub>C(b) \<sqsubseteq> P ;; Q"
-  by (metis (full_types) StateInvC_seq_idem assms seqr_mono)
-
-lemma StateInvC_extchoice_refine:
-  assumes 
-    "P is NCSP" "Q is NCSP"
-    "sinv\<^sub>C(b) \<sqsubseteq> P" "sinv\<^sub>C(b) \<sqsubseteq> Q"
-  shows "sinv\<^sub>C(b) \<sqsubseteq> P \<box> Q"
-proof -
-  have 1:
-    "pre\<^sub>R P \<sqsubseteq> [b]\<^sub>S\<^sub><" "[b]\<^sub>S\<^sub>> \<sqsubseteq> ([b]\<^sub>S\<^sub>< \<and> post\<^sub>R P)"
-    "pre\<^sub>R Q \<sqsubseteq> [b]\<^sub>S\<^sub><" "[b]\<^sub>S\<^sub>> \<sqsubseteq> ([b]\<^sub>S\<^sub>< \<and> post\<^sub>R Q)"
-    by (metis (no_types, lifting) CRR_implies_RR NCSP_implies_CSP RHS_tri_design_refine SRD_reactive_tri_design StateInvC_def assms periR_RR postR_RR preR_CRR rea_st_cond_RR rea_true_RR refBy_order st_post_CRR)+
-  show ?thesis
-    by (rdes_refine_split cls: assms(1-2), simp_all add: 1 closure assms truer_bottom_rpred  utp_pred_laws.inf_sup_distrib1)
-qed
-
 typedef ('s, 'e) Action = "{P :: ('s, 'e) action. P is CACT}"
   by (rule_tac x="Skip" in exI, simp add: closure)
 
@@ -203,31 +160,8 @@ lemma CDF_is_C2 [closure]: "CDF is C2"
 lemma CDF_is_CACT [closure]: "CDF is CACT"
   by (simp add: CACT_intro closure)
 
-definition ndiv_srd :: "('s,'t::trace,'\<alpha>) hrel_rsp" ("ndiv\<^sub>R")
-where [rdes_def]: "ndiv_srd = \<^bold>R\<^sub>s(true\<^sub>r \<turnstile> true\<^sub>r \<diamondop> true\<^sub>r)"
-
 lemma choose_srd_CACT [closure]: "ndiv\<^sub>R is CACT"
   by (simp add: rdes_def closure unrest CACT_rdes_intro)
-
-lemma ndiv_srd_refines_preR_true:
-  assumes "P is SRD"
-  shows "ndiv\<^sub>R \<sqsubseteq> P \<longleftrightarrow> pre\<^sub>R(P) = true\<^sub>r" (is "?lhs \<longleftrightarrow> ?rhs")
-proof
-  assume ?lhs
-  thus ?rhs
-    by (metis R1_preR ndiv_srd_def preR_antitone preR_rdes rea_true_RR rea_true_disj(2) utp_pred_laws.sup.orderE)    
-next
-  assume ?rhs
-  hence "ndiv\<^sub>R \<sqsubseteq> \<^bold>R\<^sub>s(pre\<^sub>R(P) \<turnstile> peri\<^sub>R(P) \<diamondop> post\<^sub>R(P))"
-    by (simp add: RHS_tri_design_conj assms ndiv_srd_def periR_SRD_R1 postR_SRD_R1 rea_true_conj(1) rea_true_impl utp_pred_laws.inf.absorb_iff2)
-  thus ?lhs
-    by (simp add: SRD_reactive_tri_design assms)
-qed
-
-lemma ndiv_srd_refines_rdes_pre_true:
-  assumes "P\<^sub>1 is RR" "P\<^sub>2 is RR" "P\<^sub>3 is RR"
-  shows "ndiv\<^sub>R \<sqsubseteq> \<^bold>R\<^sub>s(P\<^sub>1 \<turnstile> P\<^sub>2 \<diamondop> P\<^sub>3) \<longleftrightarrow> P\<^sub>1 = true\<^sub>r" (is "?lhs \<longleftrightarrow> ?rhs")
-  by (simp add: ndiv_srd_refines_preR_true closure assms rdes unrest)
 
 lift_definition divf :: "('s, 'e) Action" is "ndiv\<^sub>R"
   by (simp add: closure)
@@ -261,7 +195,7 @@ is "\<lambda> P Q R. \<^bold>R\<^sub>s(RC1(P) \<turnstile> (\<exists> $st\<acute
 lift_definition pre\<^sub>A :: "('s, 'e) Action \<Rightarrow> ('s, 'e) rrel" is "pre\<^sub>R"
   by (metis CACT_implies_NCSP NCSP_implies_NSRD NSRD_neg_pre_RC false_CDC preR_CRR wp_rea_CDC_closed wp_rea_RC_false)
 
-lift_definition StateInvA :: "'s upred \<Rightarrow> ('s, 'e) Action" ("sinv\<^sub>A") is StateInvC
+lift_definition StateInvA :: "'s upred \<Rightarrow> ('s, 'e) Action" ("sinv\<^sub>A") is StateInvR
   by (simp add: closure)
 
 lemmas action_rep_eq = 
@@ -281,7 +215,10 @@ lemmas action_rep_eq =
   contract.rep_eq
   asubst.rep_eq
   miracle.rep_eq
-  state_block_def dlockf.rep_eq state_decl.rep_eq seq.rep_eq assigns.rep_eq iteration.rep_eq 
+  state_block_def 
+  divf.rep_eq
+  dlockf.rep_eq 
+  state_decl.rep_eq seq.rep_eq assigns.rep_eq iteration.rep_eq 
   StateInvA.rep_eq
 
 subsection \<open> Action Syntax \<close>
@@ -304,7 +241,7 @@ translations
   "_skip_raction"          == "CONST skips"
   "_seq_raction P Q"       => "P ; Q"
   "_if_raction b P Q"      == "CONST cond P b Q"
-  "_assign_raction x v"    => "x := v"
+  "_assign_raction x v"    => "CONST assigns [x \<mapsto>\<^sub>s v]"
   "_basic_ev_raction e"    == "CONST sync e"
   "_rcv_ev_raction c x"    == "CONST receive c x"
   "_send_ev_raction c v"   == "CONST send c v"
@@ -362,8 +299,6 @@ lemma asubst_stop [action_simp]:
 lemma asubst_assigns [action_simp]:
   "\<sigma> \<dagger> (\<langle>\<rho>\<rangle>\<^sub>a :: ('s, 'e) Action) = \<langle>\<rho> \<circ> \<sigma>\<rangle>\<^sub>a"
   by (simp add: action_rep_eq, rdes_eq)
-
-thm usubst
 
 lemma GuardCSP_usubst:
   assumes "P is NCSP"
@@ -425,7 +360,7 @@ lemma stop_sinv_refine: "sinv\<^sub>A(a) \<sqsubseteq> stop"
 lemma extchoice_sinv_refine:
   assumes "sinv\<^sub>A(a) \<sqsubseteq> P" "sinv\<^sub>A(a) \<sqsubseteq> Q"
   shows "sinv\<^sub>A(a) \<sqsubseteq> (P \<box> Q)"
-  using assms by (transfer, simp add: CACT_implies_NCSP StateInvC_extchoice_refine)
+  using assms by (transfer, simp add: CACT_implies_NCSP extchoice_StateInvR_refine)
 
 lemma true_guard [action_simp]: "true \<^bold>& P = P"
   by (transfer, simp add: closure)
@@ -523,11 +458,6 @@ lemma asm_assign:
   using vwb_lens.put_eq apply force+
   done
 
-lemma rdes_assume_pre_refine:
-  assumes "P is NCSP"
-  shows "P \<sqsubseteq> [b]\<^sub>C ;; P"
-  by (rdes_refine cls: assms)
-
 lemma asm_pre_refine: "P \<sqsubseteq> [b]\<^sub>A ; P"
   by (simp add: action_rep_eq rdes_assume_pre_refine closure)
 
@@ -557,6 +487,42 @@ qed
 lemma dlockf_state_decl:
   "dlockf \<sqsubseteq> P \<Longrightarrow> dlockf \<sqsubseteq> state_decl P"
   by (transfer, simp add: state_srea_refine alpha)
+
+lemma divf_frame_ext:
+  "divf \<sqsubseteq> P \<Longrightarrow> divf \<sqsubseteq> a:[P]\<^sub>A\<^sup>+"
+  by (transfer, simp add: ndiv_srd_refines_preR_true closure rdes, safe, simp add: rdes_def rdes alpha closure)
+
+lemma divf_seq_refine:
+  assumes "divf \<sqsubseteq> P" "divf \<sqsubseteq> Q"
+  shows "divf \<sqsubseteq> (P ; Q)"
+  using assms by (transfer, simp add: ndiv_srd_refines_preR_true closure rdes rpred wp)
+
+lemma divf_extchoice_refine:
+  assumes "divf \<sqsubseteq> P" "divf \<sqsubseteq> Q"
+  shows "divf \<sqsubseteq> (P \<box> Q)"
+  using assms by (transfer, simp add: ndiv_srd_refines_preR_true closure rdes rpred wp)
+
+lemma divf_stop: "divf \<sqsubseteq> stop"
+  by (transfer, rdes_refine)
+
+lemma divf_extchoice_fold_refine:
+  assumes "\<And> P. P \<in> set(xs) \<Longrightarrow> divf \<sqsubseteq> P"
+  shows "divf \<sqsubseteq> foldr (op \<box>) xs stop"
+  using assms
+  apply (induct xs)
+   apply (simp_all add: divf_stop)
+  apply (rule divf_extchoice_refine)
+   apply (auto simp add: assms)
+  done
+
+lemma divf_assigns: "divf \<sqsubseteq> \<langle>\<sigma>\<rangle>\<^sub>a"
+  by (transfer, simp add: ndiv_srd_refines_preR_true closure rdes rpred wp)
+
+lemma divf_guard: "divf \<sqsubseteq> P \<Longrightarrow> divf \<sqsubseteq> b \<^bold>& P"
+  by (transfer, simp add: ndiv_srd_refines_preR_true closure rdes rpred wp)
+
+lemma divf_sync: "divf \<sqsubseteq> sync e"
+  by (transfer, simp add: ndiv_srd_refines_preR_true closure rdes rpred usubst wp)
 
 subsection \<open> Contract Theorems \<close>
 
