theories/rea_designs/utp_rdes_tactics.thy
@@ -10,7 +10,7 @@ lemmas rdes_rel_norms =
   prod.case_eq_if
   conj_assoc
   disj_assoc
-  conj_disj_distr
+  utp_pred_laws.distrib(3,4)
   conj_UINF_dist
   conj_UINF_ind_dist
   seqr_or_distl
